Add paramless to the list of constructors directly

Translation/ITyping.v
@@ -297,15 +297,15 @@ Definition isType Σ Γ A :=
   exists s, Σ ;;; Γ |-i A : sSort s.
 
 Inductive type_constructors (Σ : sglobal_context) (pars : nctx) (Γ : scontext) :
-  list (ident * sterm * nat) -> list sterm -> Type :=
-| type_cnstrs_nil : type_constructors Σ pars Γ [] []
-| type_cnstrs_cons id t t' n l l' :
+  list (ident * sterm * nat * sterm) -> Type :=
+| type_cnstrs_nil : type_constructors Σ pars Γ []
+| type_cnstrs_cons id t t' n l :
     isType Σ Γ t ->
     Xcomp t ->
-    type_constructors Σ pars Γ l l' ->
+    type_constructors Σ pars Γ l ->
     t = Prods pars t' ->
     (** TODO: check it has n products ending in a tRel application *)
-    type_constructors Σ pars Γ ((id, t, n) :: l) (t' :: l').
+    type_constructors Σ pars Γ ((id, t, n, t') :: l).
 
 Inductive type_projections (Σ : sglobal_context) (Γ : scontext) :
   list (ident * sterm) -> Type :=
@@ -325,19 +325,21 @@ Definition isArity Σ pars indices s T :=
 Inductive type_inddecls (Σ : sglobal_context) (pars : nctx) (Γ : scontext) :
   list sone_inductive_body -> Type :=
 | type_ind_nil : type_inddecls Σ pars Γ []
-| type_ind_cons na ty cstrs cstrs' projs kelim indices s l :
+| type_ind_cons na ty cstrs projs kelim indices s l :
     (** Arity is well-formed *)
     isArity Σ pars indices s ty ->
     (** TMP: The type can be written in ETT *)
     Xcomp ty ->
     (** Constructors are well-typed *)
-    type_constructors Σ pars Γ cstrs cstrs' ->
+    type_constructors Σ pars Γ cstrs ->
     (** Projections are well-typed *)
     type_projections Σ (Γ ,,, (nlctx pars) ,, ty) projs ->
     (** The other inductives in the block are well-typed *)
     type_inddecls Σ pars Γ l ->
     (** TODO: check kelim*)
-    type_inddecls Σ pars Γ (Build_sone_inductive_body na ty kelim cstrs projs indices s cstrs' :: l).
+    type_inddecls
+      Σ pars Γ
+      (Build_sone_inductive_body na ty kelim cstrs projs indices s :: l).
 
 Definition type_inductive Σ pars inds :=
   wf Σ (nlctx pars) *
